#+TITLE: MECH 366 Homework 1
#+AUTHOR: Jasper Chan - 37467164
#+OPTIONS: toc:nil
#+BEGIN_SRC ipython :session :results silent :exports none
%matplotlib inline
%config InlineBackend.figure_format = 'svg'

import SchemDraw as schem
import SchemDraw.elements as e
#+END_SRC
* 
Consider 2-DOF mass-spring-damper system in the figure below, where
$k$ $[\si{\newton/\meter}]$ is the linear spring constant,
$b_1$ $[\si{\newton\second/\meter}]$ and $b_2$ $[\si{\newton\second/\meter}]$ are viscous friction coefficients (between masses and ground),
and $b_3$ $[\si{\newton\second/\meter}]$ is the damping coefficient.
$f$ $[\si{\newton}]$ is the force input and the outputs are displacements $y_1$ $[\si{\meter}]$ and $y_1$ $[\si{\meter}]$.

#+ATTR_LATEX: :width 3in
[[file:q1.png]]

The outputs $y_1$ and $y_2$ are defined by the equations:
\begin{align}
m_1 \ddot{y}_1 &= f - k(y_1 - y_2) - b_1\dot{y}_1 - b_3(\dot{y}_1 - \dot{y}_2) \label{y1} \\
m_2 \ddot{y}_2 &= -k(y_2 - y_1) - b_2\dot{y}_2 - b_3(\dot{y}_2 - \dot{y}_1) \label{y2}
\end{align}
** 
By selecting the following states, obtain the state-space model
*** $x_1 = y_1, x_2 = \dot{y}_1, x_3 = y_2, x_4 = \dot{y}_2$ label:qb-state

We can rewrite equations (\ref{y1}) and (\ref{y2}) as:
\begin{align}
\dot{x}_2 &= \frac{1}{m_1}(u - k(x_1 - x_3) - b_1 x_2 - b_3(x_2 - x_4)) \\
\dot{x}_4 &= \frac{1}{m_2}(-k(x_3 - x_1) - b_2 x_4 - b_3(x_4 - x_2))
\end{align}

Now we can define our state-space model:
\begin{equation*}
\dot{\mathbf{x}}
=
\begin{bmatrix}
    \dot{x}_1 \\ \dot{x}_2 \\ \dot{x}_3 \\ \dot{x}_4
\end{bmatrix}
=
\begin{bmatrix}
    0 & 1 & 0 & 0 \\
    -\frac{k}{m_1} & -\frac{b_1 + b_3}{m_1} & \frac{k}{m_1} & \frac{b_3}{m_1} \\
    0 & 0 & 0 & 1 \\
    \frac{k}{m_2} & \frac{b_3}{m_2} & -\frac{k}{m_2} & -\frac{b_2 + b_3}{m_2}
\end{bmatrix}
\begin{bmatrix}
    x_1 \\ x_2 \\ x_3 \\ x_4
\end{bmatrix}
+
\begin{bmatrix}
    0 \\ \frac{1}{m_1} \\ 0 \\ 0
\end{bmatrix}
u
\end{equation*}

We can also define our output matrix:
\begin{equation*}
\mathbf{y} =
\begin{bmatrix}
    y_1 \\ y_2
\end{bmatrix}
=
\begin{bmatrix}
    1 & 0 & 0 & 0 \\
    0 & 0 & 1 & 0
\end{bmatrix}
\mathbf{x}
\end{equation*}
*** $x_1 = \dot{y}_2, x_2 = y_2, x_3 = \dot{y}_1, x_4 = y_1$
We can rewrite equations (\ref{y1}) and (\ref{y2}) as:
\begin{align}
\dot{x}_3 &= \frac{1}{m_1}(u - k(x_4 - x_2) - b_1 x_3 - b_3(x_3 - x_1)) \\
\dot{x}_1 &= \frac{1}{m_2}(-k(x_2 - x_4) - b_2 x_1 - b_3(x_1 - x_3))
\end{align}

Now we can define our state-space model:
\begin{equation*}
\dot{\mathbf{x}}
=
\begin{bmatrix}
    \dot{x}_1 \\ \dot{x}_2 \\ \dot{x}_3 \\ \dot{x}_4
\end{bmatrix}
=
\begin{bmatrix}
    -\frac{b_2 + b_3}{m_2} & -\frac{k}{m_2} & \frac{b_3}{m_2} & \frac{k}{m_2} \\
    1 & 0 & 0 & 0 \\
    \frac{b_3}{m_1} & \frac{k}{m_1} & -\frac{b_1 + b_3}{m_1} & -\frac{k}{m_1} \\
    0 & 0 & 1 & 0
\end{bmatrix}
\begin{bmatrix}
    x_1 \\ x_2 \\ x_3 \\ x_4
\end{bmatrix}
+
\begin{bmatrix}
    0 \\ 0 \\ \frac{1}{m_1} \\ 0
\end{bmatrix}
u
\end{equation*}

We can also define our output matrix:
\begin{equation*}
\mathbf{y} =
\begin{bmatrix}
    y_1 \\ y_2
\end{bmatrix}
=
\begin{bmatrix}
    0 & 0 & 0 & 1 \\
    0 & 1 & 0 & 0
\end{bmatrix}
\mathbf{x}
\end{equation*}
** 
(In this question, use the states in \ref{qb-state})
Instead of the linear spring, we assume the nonlinear spring which has the force-displacement relation of the spring as $f_z = k_1z + k_2 z^3$ (instead of the relation $f_z = kz$ for the linear spring, where $f_z$ is the force and $z$ is the displacement.
Obtain the linearized state-space model for the equilibrium point
$y_{10} = 0 [\text{m}]$,
$y_{20} = 0 [\text{m}]$ and
$\dot{y}_{10} = \dot{y}_20 = 0 [\text{m/s}]$
Also, explain the reason why the linearzation around
$\dot{y}_{10} = 1 [\text{m}]$,
$\dot{y}_{20} = 0 [\text{m}]$ and 
$\dot{y}_{10} = \dot{y}_{20} = 0 [\text{m/s}]$
is impossible.

Let's rewrite the equations (\ref{y1}) and (\ref{y2}) to fit this non-linear spring:

\begin{align}
m_1 \ddot{y}_1 &= f - f_z(y_1 - y_2) - b_1\dot{y}_1 - b_3(\dot{y}_1 - \dot{y}_2) \label{y1_2} \\
m_2 \ddot{y}_2 &= -f_z(y_2 - y_1) - b_2\dot{y}_2 - b_3(\dot{y}_2 - \dot{y}_1) \label{y2_2}
\end{align}

*** Finding the linearized state-space model
We can rewrite equations (\ref{y1_2}) and (\ref{y2_2}) with our state variables:
\begin{align}
\dot{x}_2 &= \frac{1}{m_1}(u - f_z(x_1 - x_3) - b_1 x_2 - b_3(x_2 - x_4)) \\
\dot{x}_4 &= \frac{1}{m_2}(-f_z(x_3 - x_1) - b_2 x_4 - b_3(x_4 - x_2))
\end{align}

With this, we can define our non-linear state-space model:

\begin{equation*}
\dot{\mathbf{x}}
=
\begin{bmatrix}
    x_2 \\
    \frac{1}{m_1}(u - f_z(x_1 - x_3) - b_1 x_2 - b_3(x_2 - x_4)) \\
    x_4 \\
    \frac{1}{m_2}(-f_z(x_3 - x_1) - b_2 x_4 - b_3(x_4 - x_2))
\end{bmatrix}
\end{equation*}

First, let's find our Jacobian matrices:

\begin{align*}
\mathbf{J}_{\dot{\mathbf{x}}} &= \frac{\partial \mathbf{f}}{\partial \dot{\mathbf{x}}} \\
&=
\begin{bmatrix}
    0 & 1 & 0 & 0 \\
    -\frac{k_1 + 3k_2(x_1 - x_3)^2}{m_1} &
    -\frac{b_1 + b_3}{m_1} &
    \frac{k_1 + 3k_2(x_1 - x_3)^2}{m_1} &
    \frac{b_3}{m_1} \\
    0 & 0 & 0 & 1 \\
    \frac{k_1 + 3k_2(x_1 - x_3)^2}{m_1} &
    \frac{b_3}{m_1} &
    -\frac{k_1 + 3k_2(x_1 - x_3)^2}{m_1} &
    -\frac{b_2 + b_3}{m_1} \\
\end{bmatrix} \\
\\
\mathbf{J}_\mathbf{u} &= \frac{\partial \mathbf{f}}{\partial \mathbf{u}} \\
&= 
\begin{bmatrix}
    0 \\ \frac{1}{m_1} \\ 0 \\ 0
\end{bmatrix}
\end{align*}

We can find the equilibrium input $u_0$ by subbing $\mathbf{x}_0$ into $\dot{\mathbf{x}}$

\begin{align*}
\dot{\mathbf{x}}
&=
\begin{bmatrix}
    x_2 \\
    \frac{1}{m_1}(u_0 - f_z(0) - b_1 \cdot (0) - b_3 \cdot (0)) \\
    x_4 \\
    \frac{1}{m_2}(-f_z(0) - b_2 \cdot (0) - b_3(0))
\end{bmatrix}
= 0 \\
\\
u_0 &= 0
\end{align*}

We can now find the linearized state space model matrices:
\begin{align*}
\mathbf{A} &= \left.\mathbf{J}_{\dot{\mathbf{x}}}\right|_{(\mathbf{x}_0, u_0)} \\
&=
\begin{bmatrix}
    0 & 1 & 0 & 0 \\
    -\frac{k_1}{m_1} &
    -\frac{b_1 + b_3}{m_1} &
    \frac{k_1}{m_1} &
    \frac{b_3}{m_1} \\
    0 & 0 & 0 & 1 \\
    \frac{k_1}{m_1} &
    \frac{b_3}{m_1} &
    -\frac{k_1}{m_1} &
    -\frac{b_2 + b_3}{m_1} \\
\end{bmatrix} \\
\\
\mathbf{B} &= \left.\mathbf{J}_{\mathbf{u}}\right|_{(\mathbf{x}_0, u_0)} \\
&= 
\begin{bmatrix}
    0 \\ \frac{1}{m_1} \\ 0 \\ 0
\end{bmatrix} \\
\\
\mathbf{C} &= 
\begin{bmatrix}
    0 & 0 & 0 & 1 \\
    0 & 1 & 0 & 0
\end{bmatrix}
\end{align*}

Our linearized state space model is now defined as:
\begin{align*}
\delta \dot{\mathbf{x}} &= \mathbf{A}\delta\mathbf{x} + \mathbf{B}u \\
\delta \mathbf{y} &= \mathbf{C}\delta\mathbf{x} \\
\end{align*}
*** Impossibility of $y_{10} = 1$
Because $\dot{x}_4$ does not contain a $u$ term and does not evaluate to $0$ for the given conditions, $\dot{\mathbf{x}}$ can never equal 0.




* 
Obtain a state-space model for the RLC circuit depicted below.
Here, the system has two input voltages $u_1$ and $u_2$ [V] and one output voltage [V] across the rightmost capacitor, as indicated in the figure.
$R$, $L$ and $C$ are some given constants.
(Hint: You may have some lengthy calculations.)

#+ATTR_LATEX: :width 5in
[[file:q2.png]]
First let's redraw the circuit with node names and current directions:
#+BEGIN_SRC ipython :session :results raw drawer :exports results
d = schem.Drawing()

d.add(e.SOURCE, d='up', label=['-', '$u_1$', '+'])
R1 = d.add(e.RES, d='right', label='$R/2$')
d.labelI(R1, top=False)
d.add(e.DOT, label='$1$')
R2 = d.add(e.RES, d='right', label='$R$')
d.labelI(R2, top=False)
d.add(e.DOT, label='$2$')
R3 = d.add(e.RES, d='right', label='$R$')
d.labelI(R3, top=False)
d.add(e.DOT, label='$3$')
R4 = d.add(e.RES, d='right', label='$R/2$')
d.labelI(R4, top=False)
d.add(e.SOURCE, d='down', label=['+', '$u_2$', '-'])

d.add(e.LINE, d='left')
d.push()
C1 = d.add(e.CAP2, reverse=True, d='up', label='$C$')
d.labelI(C1, top=False)
d.pop()
d.add(e.LINE, d='left')
d.push()
L1 = d.add(e.INDUCTOR, d='up', label='$L$')
d.labelI(L1, top=False)
d.pop()
d.add(e.LINE, d='left')
d.push()
C2 = d.add(e.CAP2, reverse=True, d='up', label='$C$')
d.labelI(C2, top=False)
d.pop()
d.add(e.LINE, d='left')

d.draw()

#+END_SRC

#+RESULTS:
:RESULTS:
# Out[54]:
[[file:./obipy-resources/n9ibEa.svg]]
:END:

We can now define KCL equations for each node:
\begin{align}
\text{Node 1}&: \frac{u_1 - V_1}{R/2} + C\dot{V}_1 - \frac{V_1 - V_2}{R} = 0 \\
\text{Node 2}&: \frac{V_1 - V_2}{R} + \frac{1}{L}\int{V_2 dt} - \frac{V_2 - V_3}{R} = 0 \label{node_2_0} \\
\text{Node 3}&: \frac{V_2 - V_3}{R} + C\dot{V}_3 - \frac{V_3 - u_2}{R/2} = 0
\end{align}

For the sake of brevity let's define $v_2 = \int{V_2 dt}$ such that the equations can be rewritten as:
\begin{align}
\text{Node 1}&: \frac{u_1 - V_1}{R/2} + C\dot{V}_1 - \frac{V_1 - \dot{v}_2}{R} = 0 \\
\text{Node 2}&: \frac{V_1 - \dot{v}_2}{R} + \frac{v_2}{L} - \frac{\dot{v}_2 - V_3}{R} = 0 \label{node_2_0} \\
\text{Node 3}&: \frac{\dot{v}_2 - V_3}{R} + C\dot{V}_3 - \frac{V_3 - u_2}{R/2} = 0
\end{align}

We can now choose our state variables $x_1 = V_1, x_2 = v_2, x_3 = V_3$ and rewrite our KCL equations in terms of them:
\begin{align}
\text{Node 1}&: \frac{u_1 - x_1}{R/2} + C\dot{x}_1 - \frac{x_1 - \dot{x}_2}{R} = 0 \\
\text{Node 2}&: \frac{x_1 - \dot{x}_2}{R} + \frac{x_2}{L} - \frac{\dot{x}_2 - x_3}{R} = 0 \\
\text{Node 3}&: \frac{\dot{x}_2 - x_3}{R} + C\dot{x}_3 - \frac{x_3 - u_2}{R/2} = 0
\end{align}

Let's also isolate our equations for $\dot{\mathbf{x}}$
\begin{align}
\dot{x}_1 &= \frac{1}{C}\left(-\frac{u_1 - x_1}{R/2} + \frac{x_1 - \dot{x}_2}{R} \right)\\
\dot{x}_2 &= \frac{R}{2}\left(\frac{x_1}{R} + \frac{x_2}{L} + \frac{x_3}{R} \right)\\
\dot{x}_3 &= \frac{1}{C}\left(-\frac{\dot{x}_2 - x_3}{R} + \frac{x_3 - u_2}{R/2} \right)
\end{align}

Since $\dot{x}_1$ and $\dot{x}_3$ still contain $\dot{x}_2$ terms, let's expand them out.

\begin{align}
\dot{x}_1 &= \frac{1}{C}\left(-\frac{u_1 - x_1}{R/2} + \frac{x_1}{R} - \frac{1}{2}\left(\frac{x_1}{R} + \frac{x_2}{L} + \frac{x_3}{R} \right)\right)\\
\dot{x}_2 &= \frac{R}{2}\left(\frac{x_1}{R} + \frac{x_2}{L} + \frac{x_3}{R} \right)\\
\dot{x}_3 &= \frac{1}{C}\left(-\frac{1}{2}\left(\frac{x_1}{R} + \frac{x_2}{L} + \frac{x_3}{R} \right) + \frac{x_3}{R} + \frac{x_3 - u_2}{R/2} \right)
\end{align}

Let's simplify these equations
\begin{align}
\dot{x}_1 &= \frac{5}{2RC}x_1 - \frac{1}{2LC}x_2 - \frac{1}{2RC}x_3 - \frac{2}{RC}u_1 \\
\dot{x}_2 &= \frac{1}{2}x_1 + \frac{R}{2L}x_2 + \frac{1}{2}x_3 \\
\dot{x}_3 &= -\frac{1}{2RC}x_1 - \frac{1}{2LC}x_2 + \frac{5}{2RC}x_3 - \frac{2}{RC}u_2
\end{align}

We can now define our state-space model:
\renewcommand\arraystretch{1.5}
\begin{equation*}
\dot{\mathbf{x}} =
\begin{bmatrix}
    \frac{5}{2RC} & -\frac{1}{2LC} & -\frac{1}{2RC} \\
    \frac{1}{2} & \frac{R}{2L} & \frac{1}{2}\\
    -\frac{1}{2RC} & -\frac{1}{2LC} & \frac{5}{2RC}
\end{bmatrix}
\begin{bmatrix}
    x_1 \\ x_2 \\ x_3
\end{bmatrix}
+
\begin{bmatrix}
    -\frac{1}{2RC} & 0 \\
    0 & 0 \\
    0 & -\frac{1}{2RC}
\end{bmatrix}
\begin{bmatrix}
    u_1 \\ u_2
\end{bmatrix}
\end{equation*}

We can also define our output:
\begin{equation*}
y =
\begin{bmatrix}
    0 & 0 & 1
\end{bmatrix}
\mathbf{x}
\end{equation*}

    


