#+TITLE: MECH 366 Homework 5
#+AUTHOR: Jasper Chan - 37467164
#+OPTIONS: toc:nil
#+LATEX_HEADER: \usepackage[scr]{rsfso}
#+LATEX_HEADER: \newcommand{\laplace}{\mathscr{L}}
#+LATEX_HEADER: \sisetup{per-mode=symbol}
#+LATEX_HEADER: \sisetup{inter-unit-product=\cdot}
#+BEGIN_SRC ipython :session :results silent :exports none
%matplotlib inline
%config InlineBackend.figure_format = 'svg'

from sympy import *
init_printing(use_latex=True)

def print_var(expr, var=None, mode='equation*', scale_width=False):
    output = latex(expr, mode='plain')
    if var:
        output = str(var) + "=" + output
    if scale_width:
        output = "\\resizebox{\\textwidth}{!}{$" + output + "$}"
    output = f"\\begin{{{mode}}}" + output + f"\\end{{{mode}}}"
    print(output)
    
#+END_SRC

Consider the following ordinary differential equation (ODE):
\begin{equation*}
y^{(3)}(t) + 2y^{(2)}(t) + y^{(1)}(t) = r(t)
\end{equation*}
with zero initial conditions $y(0) = y^{(1)}(0) = y^{(2)}(0) = 0$.
Here, $y^{(k)}(t)$ denotes the \(k\)-th derivative of $y(t)$.

* 
Assume that $r(t) = \delta(t)$ (i.e., unit impulse function).
** 
By using the Laplace transform, solve the ODE (i.e., obtain $y(t)$).

First let's take the Laplace transform and solve for $Y(s)$:
\begin{align*}
\laplace\left\{y^{(3)}(t) + 2y^{(2)}(t) + y^{(1)}(t)\right\}
&= \laplace\{r(t)\} \\
s^3Y(s) - \sum_{i=1}^{3}s^{(3-i)}f^{(i-1)}(0) 
+ 2\left(
    s^2Y(s) - sy(0) - y^{(1)}(0)
\right)
+ sY(s) - y(0)
&= R(s) \\
s^3Y(s) + 2s^2Y(s) + sY(s) &= 1 \\
\\
Y(s) &= \frac{1}{s^3 + 2s^2 + s} \\
&= \frac{1}{s(s + 1)^2} \\
\end{align*}

Now let's do the partial fraction expansion of $Y(s)$
\begin{align*}
Y(s) = \frac{1}{s(s + 1)^2}
&= \frac{A}{s} + \frac{B}{s + 1} + \frac{C}{(s + 1)^2} \\
1 &= A(s + 1)^2 + Bs(s + 1) + Cs \\
1 &= A(s^2 + 2s + 1) + B(s^2 + s) + Cs \\
1 &= s^2(A + B) + s(2A + B + C) + A \\
A &= 1 \\
B &= -1 \\
C &= -1 \\
\\
Y(s) &= \frac{1}{s} - \frac{1}{s + 1} - \frac{1}{(s + 1)^2} \\
\end{align*}

Now we can take the inverse Laplace transform of $Y(s)$ to find $y(t)$:
\begin{align*}
\laplace^{-1}\left\{Y(s)\right\}
&= \laplace^{-1}\left\{\frac{1}{s} - \frac{1}{s + 1} - \frac{1}{(s + 1)^2}\right\} \\
y(t) &= u(t) - e^{-t} - e^{-t}t \\
&= 1 - e^{-t} - e^{-t}t, t > 0
\end{align*}
** 
By using the final value theorem, obtain the final value $\lim_{t\to\infty}y(t)$.
(You should verify the applicability of the final value theorem.)

First, let's check the applicability of the final value theorem:
\begin{align*}
Y(s) &= \frac{1}{s(s + 1)^2} \\
\end{align*}
$Y(s)$ has one pole at $0$, and two poles at $-1$, therefore the final value theorem holds.

\begin{align*}
\lim_{t\to\infty}y(t) &= \lim_{s\to 0} sY(s) \\
&= \lim_{s\to 0} \frac{1}{(s + 1)^2} \\
&= 1
\end{align*}

* 
Next, assume that $r(t)$ is the function given in the figure below.
Note that this is an approximation of the unit impulse function.
#+ATTR_LATEX: :width 0.5\textwidth
[[file:q2.png]]
By using the final value theorem, obtain the final value $\lim_{t\to\infty}y(t)$.
(In this question, you can assume (i.e., you do not need to check) the applicability of the final value theorem.)

From the figure:
\begin{equation*}
r(t) = 2\left(u(t) - u(t - 1/2)\right)
\end{equation*}

First let's take the Laplace transform and solve for $Y(s)$:
\begin{align*}
\laplace\left\{y^{(3)}(t) + 2y^{(2)}(t) + y^{(1)}(t)\right\}
&= \laplace\{r(t)\} \\
s^3Y(s) + 2s^2Y(s) + sY(s)
&= 2\left(\frac{1}{s} - \frac{e^{-s/2}}{s}\right) \\
&= 2\left(\frac{1 - e^{-s/2}}{s}\right) \\
\\
Y(s) &= \frac{2 - 2e^{-s/2}}{s^2\left(s + 1\right)^2} \\
\end{align*}

Now let's apply the final value theorem:
\begin{align*}
\lim_{t\to\infty}y(t) &= \lim_{s\to 0} sY(s) \\
&= \lim_{s\to 0} \frac{2 - 2e^{-s/2}}{s\left(s + 1\right)^2} \\
&= \lim_{s\to 0} \frac{\frac{d}{ds}\left(2 - 2e^{-s/2}\right)}{\frac{d}{ds}\left(s\left(s + 1\right)^2\right)} \\
&= \lim_{s\to 0} \frac{e^{-s/2}}{3s^2 + 4s + 1} \\
&= 1
\end{align*}
